src/Prove.v
@@ -1,83 +1,99 @@
 Require Import Show.
 Require Import AbstractGen SetOfOutcomes Arbitrary Property.
-Require Import ssreflect.
+Require Import ssreflect ssrbool eqtype.
+
+Definition resultCorrect (r : Result) : bool := 
+  match r with
+    | MkResult (Some res) expected _ _ _ _ => 
+      res == expected
+    | _ => true
+  end.
+
+Definition failure qp :=
+  match qp with
+    | MkProp (MkRose res _) => ~~ (resultCorrect res)
+  end.
 
 Definition semProperty (P : Pred QProp) : Prop :=
   forall qp, P qp -> failure qp = false.
 
+Definition semTestable {A : Type} {_ : @Testable Pred A} (a : A) : Prop :=
+  semProperty (property a).
 
-Class Provable (A : Type) {H: Testable A} : Type :=
- {
-    semProp : A -> Prop;
-    _ : forall A, semProp A <-> semProperty (@property Pred _ _ A) 
-  }.
-
-Program Instance proveResult : Provable Result :=
-  {|
-    semProp r := 
-      match r with
-        | MkResult (Some false) _ _ _ _ _ => False 
-        | _ => True
-      end
-  |}.
-Next Obligation.
-  destruct A as [[[|] |] exp reas inter stamps callb] => /=. 
-  - split; auto. intros _. compute. 
-    by move => qp eq; subst. 
-  - split; try contradiction. 
-    set qp := 
-      {| unProp := returnRose 
-                    (MkResult (Some false) exp reas inter stamps callb) |}.
-    compute. move => /(_ qp)  H. compute in H. 
-    have contra: true = false by auto. discriminate.
-  - split; auto. intros _. compute. 
-    by move => qp eq; subst. 
-Qed.
-
-
-Program Instance proveUnit : Provable unit :=
-  {|
-    semProp := fun _ => True
-  |}.
-Next Obligation.
-  split; auto. intros _. compute. 
-  by move => qp Heq; subst.
-Qed.
-
-Program Instance proveProp : Provable QProp :=
-  {|
-    semProp qp := failure qp = false
-  |}.
-Next Obligation.
-  split. 
-  - case: A => [[res l]] //=. compute. 
-    by move => H qp Heq; subst.
-  - compute. eauto.
-Qed.
-
-Program Instance proveBool : Provable bool :=
-  {|
-    semProp b :=  b = true
-  |}.
-Next Obligation.
-  case : A.
-  - split => // _. compute. 
-    by move => qp Heq; subst.
+Lemma semBool: 
+  forall (b : bool), (b = true) <-> semTestable b.
+Proof.   
+  move => b. case: b.
+  - split => //. compute. 
+    by move => _ qp Heq; subst. 
   - split => //. compute.
     set qp := {| unProp := returnRose (updReason failed "Falsifiable") |}.
     move/(_ qp) => H. symmetry. apply H. reflexivity.
 Qed.
-  
 
-
-Lemma semForAll : forall {A prop : Type} {H : Testable prop}
-    show (gen : Pred A) (pf : A -> prop),
-  semProperty (@forAll Pred _ _ _ H show gen pf) <->
-  (forall a : A, gen a -> (semProperty (property (pf a)))).
+Lemma semResult: 
+  forall (res: Result), resultCorrect res = true <-> semTestable res.
 Proof. 
-  move => A prop Htest show gen pf. split => H'.  
-  - move => a Hgen.
-    unfold bindP, semProperty, forAll in * . move=> qp. simpl in *.
+  destruct res as [[[|] |] exp reas inter stamps callb] => /=. 
+  - split; auto. 
+    + move => /eqP Heq. compute. 
+      by move => qp eq; subst.  
+    + set qp := 
+      {| unProp := returnRose 
+                    (MkResult (Some true) exp reas inter stamps callb) |}.
+      move => /(_ qp)  H. compute in H. 
+      destruct exp. reflexivity. symmetry. by auto.  
+  - split. 
+    + move => /eqP Heq. compute. 
+      by move => qp eq; subst. 
+    + set qp := 
+      {| unProp := returnRose 
+                     (MkResult (Some false) exp reas inter stamps callb) |}.
+      move => /(_ qp)  H. compute in H. 
+      destruct exp. symmetry. by auto. reflexivity.
+  - split; auto. intros _. compute. 
+    by move => qp eq; subst. 
+Qed.
+
+Lemma semUnit: 
+  forall (t: unit), True <-> semTestable t.
+Proof.
+  move => t. split => // _. compute. 
+  by move => qp Heq; subst.
+Qed.
+
+Lemma semQProp:
+  forall (qp: QProp),
+    failure qp = false <-> semTestable qp.
+Proof.
+  move => qp. rewrite /semTestable /semProperty /property 
+                      /testProp returnGen_def. 
+  split.
+  - by move => H qp' Heq; subst.
+  - auto.
+Qed.
+
+Lemma semGen: 
+  forall (P : Type) {H : Testable P} (gen: Pred P), 
+    (forall p, gen p -> semTestable p) <-> (semTestable gen).  
+Proof.
+  move=> P H gen. split.
+  - move => H'. rewrite /semTestable /semProperty. move=> qp prop. 
+    rewrite /property /testGenProp in prop. move : prop => [p [/H' Hgen Hprop]].
+    rewrite /semTestable /semProperty in Hgen. by auto.
+  - move=> Hsem qp Hgen. rewrite /semTestable /semProperty in Hsem *.
+    move => qp' Hprop. apply Hsem. rewrite /property /testGenProp bindGen_def.
+    exists qp. split => //.
+Qed.
+   
+
+Lemma semPrintTestCase_idemp:
+  forall {prop: Type} {tp : Testable prop} (s: String.string) (p: prop),
+    semProperty (printTestCase s p) <-> semTestable p.
+Proof.
+  move => prop tp s p. rewrite /semTestable /printTestCase /semProperty. 
+  split.
+  - move => H qp Hprop. 
     set qp' :=  
       match qp with
         | {| unProp := t |} =>
@@ -87,36 +103,116 @@ Proof.
                                         (PostFinalFailure Counterexample
                                                           (fun _  _  =>
                                                              0))) t |} end.
-    move /(_ qp') : H' => H' H''. 
+    move /(_ qp') : H => H.  
     have: failure qp' = false.
-    { apply H'.  rewrite /bindP.  exists a. split => //.
-      exists qp. split => //. }
-    rewrite /qp'. destruct qp as [[[]]]. compute. auto.
-  - unfold semProperty in * => qp Hforall.
-    unfold forAllShrink in Hforall. 
-    rewrite /forAll /= /fmapP /returnP in Hforall.
-    move : Hforall => [a [Hgen [qp' [Hprop Hret]]]]. 
-    apply H' in Hprop => //. subst. 
-    destruct qp' as [[[]]]. compute. auto.
- Qed.
-
-Lemma semForAllShrink : forall {A prop : Type} {H : Testable prop}
-    show (gen : Pred A) (pf : A -> prop) shrink,
-  semProperty (@forAllShrink Pred _ _ _ H show gen shrink pf) <->
-  (forall a : A, gen a -> (semProperty (property (pf a)))).
-Proof.
-  admit.
+    { apply H.  rewrite /bindP. compute. exists qp. split => //. }
+    rewrite /qp'. destruct qp as [[[]]]. by auto.
+  - move => H qp H'. move : H' => [qp' [Hprop Hret]].
+    rewrite /returnP in Hret. apply H in Hprop. 
+    destruct qp' as [[[]]]. subst.
+    by auto.  
 Qed.
 
-Lemma forAll_forAllShrink : forall {A prop : Type} {H : Testable prop}
-    show (gen : Pred A) (pf : A -> prop) shrink,
-  semProperty (@forAllShrink Pred _ _ _ H show gen shrink pf) <->
+Lemma semBindGen: 
+  forall {A} (gen : Pred A) (p : A -> @Property Pred),
+    semProperty (bindGen gen p) <-> forall g, gen g -> semProperty (p g).
+Proof.
+  move=> A gen prop. rewrite /semProperty. split.
+  - move => H g Hgen qp Hprop. apply H. 
+    rewrite bindGen_def. exists g. split => //.
+  - move => H qp [a [Hgen Hprop]]. eauto.
+Qed.
+
+Lemma semForAll : 
+  forall {A prop : Type} {H : Testable prop} 
+         show (gen : Pred A) (pf : A -> prop),
+  (forall a : A, gen a -> (semTestable (pf a))) <->
   semProperty (@forAll Pred _ _ _ H show gen pf).
+Proof.  
+  move => A prop Htest show gen pf. split => H'.  
+  - rewrite /forAll in H' *. apply semBindGen => g Hgen.
+    rewrite semPrintTestCase_idemp. by apply H'.
+  - rewrite /forAll in H'. move/semBindGen : H' => H' a /H' Hgen.
+    by apply semPrintTestCase_idemp in Hgen.
+Qed.
+
+Lemma forAll_forAllShrink: 
+  forall {A prop : Type} {H : Testable prop}
+    show (gen : Pred A) (pf : A -> prop) shrink,
+    semProperty (@forAllShrink Pred _ _ _ H show gen shrink pf) <->
+    semProperty (@forAll Pred _ _ _ H show gen pf).
 Proof.
   admit.
 Qed.
 
-Opaque forAllShrink. 
+Lemma semForAllShrink: 
+  forall {A prop : Type} {H : Testable prop}
+         show (gen : Pred A) (pf : A -> prop) shrink,
+    (forall a : A, gen a -> (semTestable (pf a))) <-> 
+    semProperty (@forAllShrink Pred _ _ _ H show gen shrink pf).
+Proof.
+  move => A prop H show gen pf shrink.
+  rewrite forAll_forAllShrink. split; by move /semForAll => H'.
+Qed.
+
+(* I think this is the strongest property we can get for polymorphic functions *)
+Lemma semPolyFun: 
+  forall {prop : Type -> Type} {H : Testable (prop nat)} (f : forall T, prop T),
+    (semTestable (f nat)) <-> (semTestable f).
+Proof.
+  move => prop H f. rewrite /semTestable {2}/property /testPolyFun. 
+  by rewrite semPrintTestCase_idemp.
+Qed.
+
+Lemma semPolyFunSet: 
+  forall {prop : Set -> Type} {H : Testable (prop nat)} (f : forall T, prop T),
+    (semTestable (f nat)) <-> (semTestable f).
+Proof.
+  move => prop H f. rewrite /semTestable {2}/property /testPolyFun. 
+  by rewrite semPrintTestCase_idemp.
+Qed.
+
+
+Class Provable (A : Type) {H: Testable A} : Type :=
+ {
+    semProp : A -> Prop;
+    _ : forall a, semProp a <-> semTestable a 
+  }.
+
+Opaque semProp semTestable.
+
+Program Instance proveResult : Provable Result :=
+  {|
+    semProp := resultCorrect
+  |}.
+Next Obligation.
+  by apply semResult. 
+Qed.
+
+Program Instance proveUnit : Provable unit :=
+  {|
+    semProp := fun _ => True
+  |}.
+Next Obligation.
+  by apply semUnit.
+Qed.
+
+Program Instance proveQProp : Provable QProp :=
+  {|
+    semProp qp := failure qp = false
+  |}.
+Next Obligation.
+  by apply semQProp.
+Qed.
+
+Program Instance proveBool : Provable bool :=
+  {|
+    semProp b :=  b = true
+  |}.
+Next Obligation.
+  by apply semBool.
+Qed.
+
 Program Instance proveFun {A prop: Type} `{Arbitrary A} `{Show A}
         `{Provable prop}: Provable (A -> prop) :=
   {|
@@ -125,31 +221,9 @@ Program Instance proveFun {A prop: Type} `{Arbitrary A} `{Show A}
          @arbitrary _ _ Pred _ a -> 
          semProp (p a))
   |}.
-Next Obligation.
-  split. 
-  - move => H'. apply forAll_forAllShrink. 
-    destruct H2 as [proposition Proof]. destruct H1 as [property1].
-    unfold bindP, semProperty, forAll in * . move=> qp. 
-    rewrite bindGen_def. move => [a [Harb Hpr]].
-    move/(_ (A0 a)): (Proof) => Hequiv. move/Hequiv: (H' a Harb) => {Hequiv} Hequiv. 
-    move: Hpr => [qp' [/Hequiv H1 H2]]. rewrite /returnP in H2. subst.
-    by destruct qp' as [[[[|] ? ? ? ? ?] l]]. 
-  - move => /forAll_forAllShrink H' a Harb. 
-    destruct H2 as [proposition Proof]. destruct H1 as [property1].
-    unfold semProperty, semProp, forAll in * . 
-    rewrite /semProp. apply Proof. move => qp Hprop.
-    set qp' :=  match qp with
-        | {| unProp := t |} =>
-          {| unProp := fmapRose
-                         (fun r : Result =>
-                            addCallback r
-                                        (PostFinalFailure Counterexample
-                                                          (fun _  _  =>
-                                                             0))) t |} end.
-    rewrite bindGen_def in H'.
-    move /(_ qp') : H' => H'. 
-    have: failure qp' = false.
-    { apply H'.  rewrite /bindP.  exists a. split => //.
-      exists qp. split => //. }
-    rewrite /qp'. destruct qp as [[[]]]. compute. auto.
+Next Obligation. 
+ rewrite /semProp. case: H2 => semP proof. rewrite /semTestable /property /testFun.
+ split.
+ - move => H'. apply semForAllShrink => a' Hgen. apply proof. by auto.
+ - move => /semForAllShrink H' => a' Gen. apply proof. by auto.
 Qed.
